---
title: "(test post) Sampling from Dirichlet Distribution using Gamma Distributed Samples"
date: 2016-03-13
author: "Eliezer de Souza da Silva"
tags: ["old blog"]
categories: ["blog"]
---
{{< katex >}}

There is an algorithm to generate Dirichlet samples using a sampler for Gamma distribution for any \\( \alpha > 0 \\) and \\( \beta > 0 \\). We will generate Gamma distributed variables \( z_k \sim \text{gamma}(\alpha_k,1) \), for \( k \in \{1,\cdots,d\} \), and do the following variable transformation to get Dirichlet samples \( x_k = \frac{z_k}{\sum_k z_k} \). First, we should demonstrate that this transformation results in Dirichlet distributed samples.

Consider the following transformation \( (z_1,\cdots,z_d) \leftarrow (x_1,\cdots,x_d,v) \), where \( x_k = \frac{z_k}{\sum_k z_k} \) and \( v = {\sum_k z_k} \). We can rewrite this transformation as \( (x_1,\cdots,x_d,v)=h(z_1,\cdots,z_d) \), where \( x_k = \frac{z_k}{v} \) and \( v = {\sum_k z_k} \). Also, we can immediately calculate the inverse transformation \( (z_1,\cdots,z_d)=h^{-1}(x_1,\cdots,x_d,v) \), with \( z_k=v x_k \). From the transformation definition, we know that \( {\sum_{k=1}^d x_k=1} \), implying that \( x_d = 1-\sum_{k=1}^{d-1} x_k \) and \( z_d=v(1-\sum_{k=1}^{d-1}x_k) \).

Now we can apply the formula for transformation of variables to \( z_{1:d} \), \( x_{1:(d-1)} \) and \( v \) (using the notation that \( f_X \) is the pdf of the random variables \( (x_{1:(d-1)},v) \) and \( f_Z \) is the pdf of the random variables \( z_{1:d} \)):

$$
\begin{aligned}
f_{Z}(z_{1:d}) &=\prod_{k=1}^d \frac{z_k^{\alpha_k-1} e^{-z_k}}{\Gamma(\alpha_k)} \\
f_{X}(x_{1:(d-1)},v) &=f_{Z}(z_{1:d})J(z_{1:d}) \\
&=f_{Z}(h^{-1}(x_{1:(d-1)},v))\left|\frac{\partial z_{1:d}}{\partial (x_{1:(d-1)},v)}\right|
\end{aligned}
$$

So we need to compute the determinant of the Jacobian \( J(z_{1:d}) \) of the transformation.

$$
\begin{aligned}
J(z_{1:d}) &= \det \left( \begin{bmatrix}
\frac{\partial z_1}{\partial x_1} & \cdots & \frac{\partial z_1}{\partial x_{d-1}} & \frac{\partial z_1}{\partial v} \\
\frac{\partial z_2}{\partial x_1} & \cdots & \frac{\partial z_2}{\partial x_{d-1}} & \frac{\partial z_2}{\partial v} \\
\vdots & \ddots & \cdots & \vdots \\
\frac{\partial z_d}{\partial x_1} & \cdots & \frac{\partial z_d}{\partial x_{d-1}} & \frac{\partial z_d}{\partial v}
\end{bmatrix} \right)
\end{aligned}
$$

Computing the individual terms, for \( k<d \) and \( i=k \),

$$
\begin{aligned}
\frac{\partial z_k}{\partial x_i} &= \frac{\partial vx_k}{\partial x_k}\\
&=v \\
\frac{\partial z_k}{\partial v} &= \frac{\partial vx_k}{\partial v} \\
&=x_k \\
\text{for } k<d \text{ and } i \neq k\text{, }\frac{\partial z_k}{\partial x_i} &= 0 \\
\text{for } k=d \text{, }\frac{\partial z_d}{\partial x_i} &= \frac{\partial v(1-\sum_{k=1}^{d-1}x_k)}{\partial x_i} \\
&=-v \\
\frac{\partial z_d}{\partial v} &= \frac{\partial v(1-\sum_{k=1}^{d-1}x_k)}{\partial v} \\
&=1-\sum_{k=1}^{d-1}x_k
\end{aligned}
$$

In matrix form, we have:

$$
\begin{aligned}
J(z_{1:d}) &= \det \left( \begin{bmatrix}
v & 0 & 0 & \cdots & x_1 \\
0 & v & 0 & \cdots & x_2 \\
0 & 0 & v & \cdots & x_2 \\
\underset{\vdots}{0} & \underset{\vdots}{0} & \underset{\vdots}{0} & \underset{\ddots}{v} & \underset{\vdots}{x_k} \\
- v & -v & -v & \cdots & 1-\sum_{k=1}^{d-1}x_k
\end{bmatrix} \right) \\
\text{summing first line with the last line} \\
&= \det \left( \begin{bmatrix}
v & 0 & 0 & \cdots & x_1 \\
0 & v & 0 & \cdots & x_2 \\
0 & 0 & v & \cdots & x_2 \\
\underset{\vdots}{0} & \underset{\vdots}{0} & \underset{\vdots}{0} & \underset{\ddots}{v} & \underset{\vdots}{x_k} \\
0 & -v & -v & \cdots & 1+x_1-\sum_{k=1}^{d-1}x_k
\end{bmatrix} \right) \\
\text{summing all the other lines with the last line} \\
&= \det \left( \begin{bmatrix}
v & 0 & 0 & \cdots & x_1 \\
0 & v & 0 & \cdots & x_2 \\
0 & 0 & v & \cdots & x_2 \\
\underset{\vdots}{0} & \underset{\vdots}{0} & \underset{\vdots}{0} & \underset{\ddots}{v} & \underset{\vdots}{x_k} \\
0 & 0 & 0 & \cdots & 1
\end{bmatrix} \right) \\
&= v^{d-1}
\end{aligned}
$$

Now with this result from the determinant of the Jacobian, we will apply it in the transformation of random variables formula for the pdf and marginalize \( v \) to get the pdf of \( x_{1:(d-1)} \).

$$
\begin{aligned}
\Rightarrow f_{X}(x_{1:(d-1)},v) &= f_{Z}(z_{1:d}) v^{d-1} \\
&= v^{d-1} \prod_{k=1}^d \frac{{(vx_k)}^{\alpha_k-1} e^{-vx_k}}{\Gamma(\alpha_k)} \\
\Rightarrow f_{X}(x_{1:(d-1)}) &= \int_v f_{X}(x_{1:(d-1)},v) dv \\
&= \prod_{k=1}^d \frac{x_k^{\alpha_k-1}}{\Gamma(\alpha_k) } \int_v v^{d-1} \prod_{k=1}^d v^{\alpha_k-1} e^{-vx_k} dv \\
&= \prod_{k=1}^d \frac{x_k^{\alpha_k-1}}{\Gamma(\alpha_k) } \int_v v^{d-1-d+\sum_k \alpha_k} e^{-v \sum_k x_k} dv \\
&= \prod_{k=1}^d \frac{x_k^{\alpha_k-1}}{\Gamma(\alpha_k) } \underbrace{\int_v v^{-1+\sum_k \alpha_k} e^{-v} dv}_{\Gamma(\sum_k \alpha_k)} \\
\Rightarrow f_{X}(x_{1:(d-1)}) &= \Gamma(\sum_k \alpha_k) \prod_{k=1}^d \frac{x_k^{\alpha_k-1}}{\Gamma(\alpha_k)} \square \\
\end{aligned}
$$

This finishes our demonstration that the given transformation of Gamma distributed random variables results in Dirichlet distributed random variables. Notice that \( x_d \) is totally determined by \( x_{1:(d-1)} \) (\( \sum_k x_k = 1 \)), so we can actually express the right side of the equation as a formula of only \( x_{1:(d-1)} \).

If drawing \( d \) samples from a Gamma distribution can be performed with complexity \( O(g(d)) \), then \( d \) samples from a Dirichlet distribution can be computed with the same \( O(g(d)) \) complexity.
